Loda/TypingTest.lean
@@ -1,0 +1,25 @@
+import Loda.Ast
+import Loda.Typing
+
+open Ast
+-- dummy environments
+def σ0 : Env := fun _ => Value.vBool true
+def Γ0 : TyEnv := fun _ => (Ty.refin (Value.vBool true) Ty.bool (True))
+def Γ1 := setTy Γ0 "x" Ty.bool
+def δ0 : Ast.CircuitEnv :=
+  fun _ => { name := "idInt", inputs := [("x", Ast.Ty.int)], output := Ast.Ty.int,
+                 body := Ast.Expr.var "x" }
+
+example : SubtypeJudgment σ0 Γ0 (pure Ty.int) (pure Ty.int) :=
+  SubtypeJudgment.TSub_Refl
+
+-- refinement subtyping: {v:int | True} <: {v:int | True}
+example : SubtypeJudgment σ0 Γ0 (pure (Ty.refin (Value.vInt 1) Ty.int (True))) (pure (Ty.refin (Value.vInt 1) Ty.int (True))) := by
+  apply SubtypeJudgment.TSub_Refine
+  · apply SubtypeJudgment.TSub_Refl
+  · intros _; trivial
+
+-- TE_VAR: assume env maps "b" to {v | v = eval ...}
+example : TypeJudgment σ0 δ0 Γ0 123 (Expr.var "b") ((Ty.refin (Value.vBool true) Ty.bool (Value.vBool true = eval σ0 δ0 123 (Expr.var "b"))), σ0) := by
+  apply TypeJudgment.TE_Var
+  simp [Γ0]
